lambda2Gmu/Prelude.v
@@ -30,7 +30,7 @@ Ltac gather_vars :=
   let F := gather_vars_with (fun x : ctx => dom x \u fv_env x) in
   let G := gather_vars_with (fun x : list var => from_list x) in
   let H := gather_vars_with (fun x : list typ => fv_typs x) in
-  let I := gather_vars_with (fun x : typctx => domΔ x) in
+  let I := gather_vars_with (fun x : typctx => domΔ x \u fv_delta x) in
   constr:(A \u B \u C \u E \u F \u G \u H \u I).
 
 (** "pick_fresh x" tactic create a fresh variable with name x *)
